testdata/modules/crossmod_diamond/_cache/mod/extract/b.example/pb@v0.1.0/pb.cue
@@ -1,0 +1,7 @@
+package pb
+
+import "c.example/pc"
+
+#B: {
+	c: pc.#C
+}
