testdata/modules/crossmod_diamond/cue.mod/module.cue
@@ -1,0 +1,12 @@
+module: "app.example"
+language: {
+	version: "v0.15.4"
+}
+deps: {
+	"a.example/pa@v0": {
+		v: "v0.1.0"
+	}
+	"b.example/pb@v0": {
+		v: "v0.1.0"
+	}
+}
